SN_P.v
@@ -12,16 +12,16 @@ Import PSem PSyn.
 Module SNP := Abs_SN_Theory PresburgerTheory PresburgerSem IntpPresburger.
 
 Import SNP.
-Import Esub SN_CC_Real.
+Import SN_CC_Real.
 Import SN.
 Import PresburgerTheory PresburgerSem IntpPresburger.
 
 Lemma SN_P : forall e x y,
-  (exists hyp a b i j, 
-    x = app_esub i j (intp_foterm a) /\
-    y = app_esub i j (intp_foterm b) /\
+  (exists hyp a b s, 
+    x = Sub (intp_foterm a) s /\
+    y = Sub (intp_foterm b) s /\
     wf_clsd_env (intp_hyp hyp) /\
-    typ_esub e i j (intp_hyp hyp) /\
+    typ_sub e s (intp_hyp hyp) /\
     deriv hyp (eq_foterm a b)) ->
   eq_typ e x y.
 Proof. apply SN_T. Qed.
